src/tls/Negotiation.Version.fst
@@ -1,0 +1,365 @@
+module Negotiation.Version
+
+open Parsers.ProtocolVersion
+open Parsers.ClientHelloExtension
+open TLSConstants // for leqPV and the configuration
+
+open FStar.Error
+open TLSError
+
+// updated excerpts of Negotiation re: protocol versions
+
+/// ---- PROTOCOL VERSIONS ----
+///
+/// The protocol version is negotiated in ClientHello and ServerHello,
+/// using two overlapping mechanisms.  We currently implement only TLS
+/// 1.2 and 1.3, and the negotiated version can be further constrained
+/// in the connection initial configuration.
+
+// 19-01-04 TODO? 
+// * replace min/max_version in config with the payload of the supported_version extension.
+// * refine TLSConstants.protocolVersion with implemented instead of not Unknown. 
+
+let implemented pv =
+  pv = TLS_1p2 || pv = TLS_1p3
+
+let (<=) = leqPV
+
+let supported cfg pv =
+  implemented pv &&
+  cfg.min_version <= pv && pv <= cfg.max_version
+
+// negotiation failures; unnecessary?
+// private let illegal       #a msg: result a = fatal #a Illegal_parameter msg
+// private let unsupported   #a msg: result a = fatal #a Unsupported_extension msg
+// private let fatal_version #a msg: result a = fatal #a Protocol_version msg
+
+/// (1) Client offers supported versions
+///
+/// Offer only locally-implemented versions, irrespective of the
+/// configuration. We may provide more flexible configurations by replacing
+/// min/max_version with a list of supported versions.
+
+#push-options "--query_stats --z3rlimit 100" // 19-01-04 too slow? note the refinement on the length of the inner lists. 
+(*
+let offer_versions cfg: option clientHelloExtension =
+  match cfg.min_version, cfg.max_version with
+  | TLS_1p3, TLS_1p3 -> Some (CHE_supported_versions [TLS_1p3])
+  | TLS_1p2, TLS_1p3 -> Some (CHE_supported_versions [TLS_1p3; TLS_1p2])
+  | TLS_1p2, TLS_1p2 -> Some (CHE_supported_versions [TLS_1p2])
+  | _                -> None
+*)
+
+// Alternative code, easier to refine and extract; worth the trouble? 
+private let cons_supported cfg pv pvs = if supported cfg pv then pv::pvs else pvs 
+let support cfg: result clientHelloExtension =
+  let vs = cons_supported cfg TLS_1p2 [] in 
+  let vs = cons_supported cfg TLS_1p3 vs in 
+  if List.isEmpty vs 
+  then fatal Internal_error "configuration must include a supported protocol version"
+  else Correct (CHE_supported_versions vs)
+#pop-options
+
+(* too large?
+let same_supported cfg: Lemma (supported_versions cfg == supported_versions2 cfg) =
+  match cfg.min_version, cfg.max_version with
+  | SSL_3p0, SSL_3p0 -> assert_norm (supported_versions cfg == supported_versions2 cfg)
+  | SSL_3p0, TLS_1p0 -> assert_norm (supported_versions cfg == supported_versions2 cfg)
+  | SSL_3p0, TLS_1p1 -> assert_norm (supported_versions cfg == supported_versions2 cfg)
+  | SSL_3p0, TLS_1p2 -> assert_norm (supported_versions cfg == supported_versions2 cfg)
+  | SSL_3p0, TLS_1p3 -> assert_norm (supported_versions cfg == supported_versions2 cfg)
+  | TLS_1p0, SSL_3p0 -> assert_norm (supported_versions cfg == supported_versions2 cfg)
+  | TLS_1p0, TLS_1p0 -> assert_norm (supported_versions cfg == supported_versions2 cfg)
+  | TLS_1p0, TLS_1p1 -> assert_norm (supported_versions cfg == supported_versions2 cfg)
+  | TLS_1p0, TLS_1p2 -> assert_norm (supported_versions cfg == supported_versions2 cfg)
+  | TLS_1p0, TLS_1p3 -> assert_norm (supported_versions cfg == supported_versions2 cfg)
+  | TLS_1p1, SSL_3p0 -> assert_norm (supported_versions cfg == supported_versions2 cfg)
+  | TLS_1p1, TLS_1p0 -> assert_norm (supported_versions cfg == supported_versions2 cfg)
+  | TLS_1p1, TLS_1p1 -> assert_norm (supported_versions cfg == supported_versions2 cfg)
+  | TLS_1p1, TLS_1p2 -> assert_norm (supported_versions cfg == supported_versions2 cfg)
+  | TLS_1p1, TLS_1p3 -> assert_norm (supported_versions cfg == supported_versions2 cfg)
+  | TLS_1p2, SSL_3p0 -> assert_norm (supported_versions cfg == supported_versions2 cfg)
+  | TLS_1p2, TLS_1p0 -> assert_norm (supported_versions cfg == supported_versions2 cfg)
+  | TLS_1p2, TLS_1p1 -> assert_norm (supported_versions cfg == supported_versions2 cfg)
+  | TLS_1p2, TLS_1p2 -> assert_norm (supported_versions cfg == supported_versions2 cfg)
+  | TLS_1p2, TLS_1p3 -> assert_norm (supported_versions cfg == supported_versions2 cfg)
+  | TLS_1p3, SSL_3p0 -> assert_norm (supported_versions cfg == supported_versions2 cfg)
+  | TLS_1p3, TLS_1p0 -> assert_norm (supported_versions cfg == supported_versions2 cfg)
+  | TLS_1p3, TLS_1p1 -> assert_norm (supported_versions cfg == supported_versions2 cfg)
+  | TLS_1p3, TLS_1p2 -> assert_norm (supported_versions cfg == supported_versions2 cfg)
+  | TLS_1p3, TLS_1p3 -> assert_norm (supported_versions cfg == supported_versions2 cfg)
+*)
+
+/// (2) Server chooses a supported version
+///
+/// Check that the protocol version in ClientHello is within the
+/// range of versions supported by the server configuration and
+/// outputs the negotiated version if true
+
+// temporary; will use Parsers.ClientHello.clientHello 
+type ch = HandshakeMessages.ch
+private let offered_version o = o.HandshakeMessages.ch_protocol_version 
+private let offered_extensions o = o.HandshakeMessages.ch_extensions 
+
+// We ignore the "minimal protocol version" signalled in the packet
+// header; this is fine since our server never accepts any proposal
+// below the "maximal protocol version".
+
+private let correct #a (x:a): result a = Correct x
+ 
+#set-options "--z3rlimit 100"
+val choose: cfg:config -> ch -> result (pv:protocolVersion{ supported cfg pv })
+let choose cfg ch =
+  let legacy_max_pv = offered_version ch in // offer.Parsers.ClientHello.version in
+  if TLS_1p3 <= legacy_max_pv then
+    fatal Protocol_version "protocol version negotiation: bad legacy proposal"
+  else
+    match List.Tot.find CHE_supported_versions? (offered_extensions ch) with
+    | None ->
+      // legacy negotiation: we pick at most TLS 1p2
+      if legacy_max_pv = TLS_1p2 && supported cfg TLS_1p2 then
+        correct TLS_1p2
+      else
+        fatal Protocol_version "protocol version negotiation: mismatch"
+
+    | Some (CHE_supported_versions vs) ->
+      // new extension-based negotiation: we pick the first client offer supported by the server
+      match List.Helpers.find_aux cfg supported vs with
+      | Some v -> correct v
+      | None -> fatal Protocol_version "protocol version negotiation: mismatch"
+#reset-options
+
+/// (3) Client validates the server's choice
+
+(**
+  Determines if the server random value contains a downgrade flag
+  AND if there has been a downgrade
+  The downgrade flag is a random value set by RFC (6.3.1.1)
+*)
+val isSentinelRandomValue:
+  Parsers.ProtocolVersion.protocolVersion ->
+  Parsers.ProtocolVersion.protocolVersion ->
+  TLSInfo.random ->
+  bool
+let isSentinelRandomValue client_pv server_pv server_random =
+  let open FStar.Bytes in
+  let down = bytes_of_string "DOWNGRD" in
+  assume(length down = 7 /\ length (abyte 1z) = 1 /\ length (abyte 0z) = 1); //18-12-16 TODO how?
+  (server_pv <= TLS_1p2 && TLS_1p3 <= client_pv && server_random = down @| abyte 1z) ||
+  (server_pv <= TLS_1p1 && TLS_1p2 <= client_pv && server_random = down @| abyte 0z)
+
+val accept:
+  cfg: config ->
+  pv: protocolVersion ->
+  ses: Parsers.ServerHello_extensions.serverHello_extensions ->
+  sr: TLSInfo.random ->
+  result (pv: Parsers.ProtocolVersion.protocolVersion{ supported cfg pv })
+
+// 18-12-23 separate protocol-version negotiation, usable as spec & implementation.
+
+#set-options "--z3rlimit 100"
+let accept cfg pv ses sr =
+  if pv = TLS_1p3 then
+    fatal Illegal_parameter "cannot negotiate TLS 1.3 explicitly"
+  else
+    let open Parsers.ServerHelloExtension in
+    let chosen: Parsers.ProtocolVersion.protocolVersion (*may be unknown*) =
+      match List.Tot.find SHE_supported_versions? ses with
+      | None -> pv // old style
+      | Some (SHE_supported_versions pv) -> pv in
+    if TLS_1p3 <= chosen && pv <> TLS_1p2 then
+      fatal Illegal_parameter "extension-based version negotiation requires TLS 1.2 apparent version"
+    else
+    if isSentinelRandomValue cfg.max_version chosen sr then 
+      fatal Illegal_parameter "protocol-version downgrade attempt"
+    else 
+    if not (supported cfg chosen) then 
+      fatal Illegal_parameter "client did not offer this protocol version"
+    else
+      correct chosen
+#reset-options
+
+(* BEYOND VERSIONS 
+
+/// ----
+///
+/// server's handling of ClientHello, a rather long stateful function.
+/// calling (pure) computeServerMode, then the application callback. 
+///
+ 
+let find_client_extension (filter:clientHelloExtension -> bool) o
+  : option (e:clientHelloExtension{filter e}) =
+  List.Tot.find filter o.Parsers.ClientHello.extensions 
+
+let find_client_key_shares (o:offer): Parsers.KeyShareClientHello.keyShareClientHello =
+  match find_client_extension CHE_key_share? o with
+  | Some (CHE_key_share x) -> x
+  | _ -> assume(Parsers.KeyShareClientHello.keyShareClientHello_list_bytesize [] = 0); []
+//TODO 19-01-04 where to get it from? 
+
+let group_of_hrr hrr : option CommonDH.group = None
+//19-01-03 TODO where are QD's HRR extensions? 
+(*
+  match List.Tot.find (Extensions.E_key_share?) hrr.hrr_extensions with
+  | Some (Extensions.E_key_share (CommonDH.HRRKeyShare ng)) ->
+    CommonDH.group_of_namedGroup ng
+  | _ -> None
+*)
+
+private
+let sameExtensionTag e0 e1 = tag_of_clientHelloExtension e0 = tag_of_clientHelloExtension e1 
+
+private
+let retry_extension_ok (o1, hrr) (e:clientHelloExtension) = 
+  match e with
+// 19-01-04 TODO   
+// | Case_key_share shares2 -> (
+//     match shares2, group_of_hrr hrr with
+//     | [CommonDH.Share g _], Some g' -> g = g'
+//     | _, None ->
+//         let shares1 = find_client_key_shares o1 in
+//         //TODO 19-01-03 easier on the underlying wire representation
+//         Parsers.KeyShareClientHello.keyShareClientHello_serializer32 shares1 =
+//         Parsers.KeyShareClientHello.keyShareClientHello_serializer32 shares2
+//         // CommonDH.clientKeyShareBytes shares1 = CommonDH.clientKeyShareBytes shares2
+//     | _ -> false)
+  | CHE_early_data _ -> false // Forbidden
+  | CHE_cookie c -> true // FIXME we will send cookie
+      // If we add cookie support we need to treat this case separately
+      // | Extensions.E_cookie c -> c = S_HRR?.cookie ns.state
+  | e ->
+        (match List.Helpers.find_aux e sameExtensionTag o1 with
+        | None -> (IO.debug_print_string "Extra extension\n") && false
+        // This allows the client to send less extensions,
+        // but the ones that are sent must be exactly the same
+        | Some e' ->
+          //FIXME: Extensions.E_pre_shared_key "may be updated" 4.1.2
+          true) // FIXME
+          //(extensionBytes e) = (extensionBytes e'))
+
+// check the second offer is compatible with the first (see RFC)
+let retry_offer_ok o1 hrr o2 = 
+  let open Parsers.ClientHello in 
+  o1.version = o2.version &&
+  o1.random = o2.random &&
+  o1.session_id = o2.session_id &&
+// TODO 19-01-04 
+//  o1.session_id = hrr.hrr_sessionID &&
+//  List.Tot.mem hrr.hrr_cipher_suite o2.ch_cipher_suites &&
+  o1.compression_method = o2.compression_method &&
+  List.Helpers.forall_aux (o1.extensions, hrr) retry_extension_ok o2.extensions
+
+
+(*
+// typeckecks but yields unsafe C.
+let small (a:option (list bool)) = None? a || List.length (Some?.v a) < 10
+
+// uglier, yields good C, possible recommended style in Low*
+let small2 (a:option (list bool)) = 
+  if None? a then true else List.length (Some?.v a) < 10
+
+// we miss an early inlining semantics to get both with [let ( || ) = if a then true else b]
+*)
+
+(*
+open Mem 
+
+val server_ClientHello: // #region:rgn -> t region Server ->
+  offer -> // log:HandshakeLog.t ->
+  St (result serverMode)
+#set-options "--admit_smt_queries true"
+let server_ClientHello #region ns offer log =
+  trace ("offered client extensions "^string_of_option_extensions offer.ch_extensions);
+  trace ("offered cipher suites "^(string_of_ciphersuitenames offer.ch_cipher_suites));
+  trace (match (offered_versions TLS_1p0 offer) with
+        | Error z -> "Error: "^string_of_error z
+        | Correct v -> List.Tot.fold_left accum_string_of_pv "offered versions" v);
+  match !ns.state with
+  | S_HRR o1 hrr ->
+    trace ("Processing second offer based on existing HRR state (stateful HRR).");
+    if retry_offer_ok o1 offer
+    then
+      let sm = computeServerMode ns.cfg offer ns.nonce in
+      match sm with
+      | Error z ->
+        trace ("negotiation failed: "^string_of_error z);
+        Error z
+      | Correct (ServerHelloRetryRequest hrr _) ->
+        fatal Illegal_parameter "client sent the same hello in response to hello retry"
+      | Correct (ServerMode m cert _) ->
+        trace ("negotiated after HRR "^string_of_pv m.n_protocol_version^" "^string_of_ciphersuite m.n_cipher_suite);
+        let nego_cb = ns.cfg.nego_callback in
+        let exts_bytes = Extensions.app_extensions_bytes offer.ch_extensions in
+        trace ("Negotiation callback to handle extra extensions.");
+        match nego_cb.negotiate nego_cb.nego_context m.n_protocol_version exts_bytes (Some empty_bytes) with
+        | Nego_accept sexts ->
+          let el = Extensions.ext_of_custom sexts in
+          ns.state := S_ClientHello m cert;
+          Correct (ServerMode m cert el)
+        | _ ->
+          trace ("Application requested to abort the handshake after internal HRR.");
+          fatal Handshake_failure "application aborted the handshake by callback"
+    else
+      fatal Illegal_parameter "Inconsistant parameters between first and second client hello"
+
+  | S_Init _ ->
+    let sm = computeServerMode ns.cfg offer ns.nonce in
+    let previous_cookie = // for stateless HRR
+      match find_cookie offer with
+      | None -> None
+      | Some c ->
+        match Ticket.check_cookie c with
+        | None -> trace ("WARNING: ignorning invalid cookie "^(hex_of_bytes c)); None
+        | Some (hrr, digest, extra) ->
+          trace ("Loaded stateless retry cookie "^(hex_of_bytes c));
+          let hrr = { hrr with hrr_extensions =
+            (Extensions.E_cookie c) :: hrr.hrr_extensions; } in
+          // Overwrite the current transcript digest with values from cookie
+          trace ("Overwriting the transcript digest with CH1 hash "^(hex_of_bytes digest));
+          HandshakeLog.load_stateless_cookie log hrr digest;
+          Some extra // for the server nego callback
+      in
+    match sm with
+    | Error z ->
+      trace ("negotiation failed: "^string_of_error z);
+      Error z
+    | Correct (ServerHelloRetryRequest hrr cs) ->
+      // Internal HRR caused by group negotiation
+      // We do not invoke the server nego callback in this case
+      // record the initial offer and return the HRR to HS
+      let ha = verifyDataHashAlg_of_ciphersuite cs in
+      let digest = HandshakeLog.hash_tag #ha log in
+      let cookie = Ticket.create_cookie hrr digest empty_bytes in
+      let hrr = { hrr with hrr_extensions =
+        (Extensions.E_cookie cookie) :: hrr.hrr_extensions; } in
+      ns.state := S_HRR offer hrr;
+      sm
+    | Correct (ServerMode m cert _) ->
+      let nego_cb = ns.cfg.nego_callback in
+      let exts_bytes = Extensions.app_extensions_bytes offer.ch_extensions in
+      trace ("Negotiation callback to handle extra extensions and query for stateless retry.");
+      trace ("Application data in cookie: "^(match previous_cookie with | Some c -> hex_of_bytes c | _ -> "none"));
+      match nego_cb.negotiate nego_cb.nego_context m.n_protocol_version exts_bytes previous_cookie with
+      | Nego_abort ->
+        trace ("Application requested to abort the handshake.");
+        fatal Handshake_failure "application aborted the handshake by callback"
+      | Nego_retry cextra ->
+        let hrr = ({
+          hrr_sessionID = offer.ch_sessionID;
+          hrr_cipher_suite = name_of_cipherSuite m.n_cipher_suite;
+          hrr_extensions = [
+            Extensions.E_supported_versions (Extensions.ServerPV TLS_1p3);
+          ]}) in
+        let ha = verifyDataHashAlg_of_ciphersuite m.n_cipher_suite in
+        let digest = HandshakeLog.hash_tag #ha log in
+        let cookie = Ticket.create_cookie hrr digest cextra in
+        let hrr = { hrr with hrr_extensions =
+          (Extensions.E_cookie cookie) :: hrr.hrr_extensions; } in
+        ns.state := (S_HRR offer hrr);
+        Correct (ServerHelloRetryRequest hrr m.n_cipher_suite)
+      | Nego_accept sexts ->
+        trace ("negotiated "^string_of_pv m.n_protocol_version^" "^string_of_ciphersuite m.n_cipher_suite);
+        ns.state := S_ClientHello m cert;
+        Correct (ServerMode m cert (Extensions.ext_of_custom sexts))
+*)
+*)
